Lean4Lean/Verify/Environment/Extension.lean
@@ -12,11 +12,7 @@ theorem TrEnv.exists_addConst (H : TrEnv safety env venv) (hn : env.find? name =
   unfold VEnv.addConst
   cases hfind : venv.constants name with
   | none => simp
-  | some ci =>
-    exfalso
-    obtain ⟨ci, hci, _⟩ := H.find?_iff.2 ⟨ci, hfind⟩
-    rw [hn] at hci
-    contradiction
+  | some ci => obtain ⟨ci, hci, _⟩ := H.find?_iff.2 ⟨ci, hfind⟩; cases hn ▸ hci
 
 theorem TrEnv'.no_inductInfo (H : TrEnv' .unsafe C Q venv) :
     C.find? name ≠ some (.inductInfo info) := by
@@ -25,28 +21,11 @@ theorem TrEnv'.no_inductInfo (H : TrEnv' .unsafe C Q venv) :
   | ignore hn hhidden H ih =>
     rename_i C' Q' env' ci
     exact False.elim <| hhidden (by cases ci.safety <;> rfl)
-  | «axiom» htr hn hwf hadd H ih =>
-    rw [H.map_wf.find?_insert]
-    split
-    · simp
-    · exact ih
-  | defn htr hn hwf hadd H ih =>
-    rw [H.map_wf.find?_insert]
-    split
-    · simp
-    · exact ih
-  | thm htr hn hwf hprop hadd H ih =>
-    rw [H.map_wf.find?_insert]
-    split
-    · simp
-    · exact ih
-  | «opaque» htr hn hwf hadd H ih =>
-    rw [H.map_wf.find?_insert]
-    split
-    · simp
-    · exact ih
+  | «axiom» _ _ _ _ H ih => rw [H.map_wf.find?_insert]; split <;> [simp; exact ih]
+  | defn _ _ _ _ H ih => rw [H.map_wf.find?_insert]; split <;> [simp; exact ih]
+  | thm _ _ _ _ _ H ih => rw [H.map_wf.find?_insert]; split <;> [simp; exact ih]
+  | «opaque» _ _ _ _ H ih => rw [H.map_wf.find?_insert]; split <;> [simp; exact ih]
   | quot hready hadd H ih =>
-    dsimp [AddQuot, AddQuot1] at hadd
     obtain ⟨lp₁, ty₁, env₁, _, hn₁, _,
       lp₂, ty₂, env₂, _, hn₂, _,
       lp₃, ty₃, env₃, _, hn₃, _,
@@ -58,20 +37,11 @@ theorem TrEnv'.no_inductInfo (H : TrEnv' .unsafe C Q venv) :
       (.quotInfo { name := ``Quot.mk, kind := .ctor, levelParams := lp₂, type := ty₂ }) hn₂
     have wf₃ := wf₂.insert ``Quot.lift
       (.quotInfo { name := ``Quot.lift, kind := .lift, levelParams := lp₃, type := ty₃ }) hn₃
-    rw [wf₃.find?_insert]
-    split
-    · simp
-    rw [wf₂.find?_insert]
-    split
-    · simp
-    rw [wf₁.find?_insert]
-    split
-    · simp
-    rw [wf₀.find?_insert]
-    split
-    · simp
-    exact ih
-  | induct _ hadd _ _ => exact nomatch hadd
+    rw [wf₃.find?_insert]; split <;> [simp; skip]
+    rw [wf₂.find?_insert]; split <;> [simp; skip]
+    rw [wf₁.find?_insert]; split <;> [simp; skip]
+    rw [wf₀.find?_insert]; split <;> [simp; exact ih]
+  | induct _ hadd => cases hadd
 
 theorem VEnv.addConst_mono {env₁ env₂ env₁' env₂' : VEnv} (H : env₁ ≤ env₂)
     (h₁ : env₁.addConst name ci = some env₁') (h₂ : env₂.addConst name ci = some env₂') :
@@ -79,20 +49,13 @@ theorem VEnv.addConst_mono {env₁ env₂ env₁' env₂' : VEnv} (H : env₁ �
   unfold VEnv.addConst at h₁ h₂
   split at h₁ <;> cases h₁
   split at h₂ <;> cases h₂
-  constructor
-  · intro n a ha
-    simp at ha ⊢
-    split at ha <;> split <;> simp_all
-    exact H.constants ha
-  · exact H.defeqs
+  refine { constants {n a} := ?_, defeqs := H.defeqs }
+  dsimp; split <;> [exact id; exact H.constants]
 
 theorem VEnv.addDefEq_mono {env₁ env₂ : VEnv} (H : env₁ ≤ env₂) :
-    env₁.addDefEq df ≤ env₂.addDefEq df := by
-  constructor
-  · exact H.constants
-  · rintro d (rfl | hd)
-    · exact .inl rfl
-    · exact .inr (H.defeqs hd)
+    env₁.addDefEq df ≤ env₂.addDefEq df where
+  constants := H.constants
+  defeqs := by rintro d (rfl | hd) <;> [exact .inl rfl; exact .inr (H.defeqs hd)]
 
 theorem VEnv.addConst_eq_of_ne
     {env env' : VEnv}
@@ -106,92 +69,64 @@ theorem VEnv.HasPrimitives.addConst {env env' : VEnv} (H : env.HasPrimitives)
     (hname : Environment.primitives.contains name = false)
     (hadd : env.addConst name ci = some env') : env'.HasPrimitives := by
   have le := VEnv.addConst_le hadd
-  have same (n : Name) (hp : Environment.primitives.contains n = true) :
+  have same {n} (hp : Environment.primitives.contains n = true) :
       env'.constants n = env.constants n :=
     VEnv.addConst_eq_of_ne hadd fun h => by subst h; simp_all
-  have oldContains (n : Name) (hp : Environment.primitives.contains n = true) :
-      env'.contains n → env.contains n := by
-    rintro ⟨ci, hci⟩
-    exact ⟨ci, (same n hp) ▸ hci⟩
-  have newContains (n : Name) : env.contains n → env'.contains n := by
-    rintro ⟨ci, hci⟩
-    exact ⟨ci, le.constants hci⟩
-  let prims := [
-    ``Bool, ``Bool.false, ``Bool.true,
-    ``Nat, ``Nat.zero, ``Nat.succ,
-    ``Nat.add, ``Nat.pred, ``Nat.sub, ``Nat.mul, ``Nat.pow,
-    ``Nat.gcd, ``Nat.mod, ``Nat.div, ``Nat.beq, ``Nat.ble,
-    ``Nat.bitwise, ``Nat.land, ``Nat.lor, ``Nat.xor,
-    ``Nat.shiftLeft, ``Nat.shiftRight,
-    ``String.ofList, ``Char.ofNat]
-  have hprims : Environment.primitives = .ofList prims := rfl
-  replace hprims {n} : Environment.primitives.contains n ↔ n ∈ prims := by
+  have oldContains {n} (hp : Environment.primitives.contains n = true) :
+      env'.contains n → env.contains n := fun ⟨ci, hci⟩ => ⟨ci, (same hp) ▸ hci⟩
+  have newContains {n} : env.contains n → env'.contains n := fun ⟨ci, hci⟩ => ⟨ci, le.constants hci⟩
+  refine let prims := _; have hprims : Environment.primitives = .ofList prims := rfl; ?_
+  replace hprims {n} : n ∈ prims → Environment.primitives.contains n := by
     simp [hprims, NameSet.contains, NameSet.ofList]
-  have primBool : Environment.primitives.contains ``Bool = true := hprims.2 (by simp [prims])
-  have primBoolFalse : Environment.primitives.contains ``Bool.false = true :=
-    hprims.2 (by simp [prims])
-  have primBoolTrue : Environment.primitives.contains ``Bool.true = true :=
-    hprims.2 (by simp [prims])
-  have primNat : Environment.primitives.contains ``Nat = true := hprims.2 (by simp [prims])
-  have primNatZero : Environment.primitives.contains ``Nat.zero = true :=
-    hprims.2 (by simp [prims])
-  have primNatSucc : Environment.primitives.contains ``Nat.succ = true :=
-    hprims.2 (by simp [prims])
-  have prim (n : Name) (h : n ∈ [``Nat.add, ``Nat.sub, ``Nat.mul, ``Nat.pow, ``Nat.gcd,
-      ``Nat.mod, ``Nat.div, ``Nat.beq, ``Nat.ble, ``Nat.land, ``Nat.lor, ``Nat.xor,
-      ``Nat.shiftLeft, ``Nat.shiftRight, ``Char.ofNat, ``String.ofList]) :
-      Environment.primitives.contains n = true := by
-    simp at h
-    rcases h with rfl | rfl | rfl | rfl | rfl | rfl | rfl | rfl | rfl | rfl | rfl |
-      rfl | rfl | rfl | rfl | rfl <;> exact hprims.2 (by simp [prims])
+  simp only [List.mem_cons, prims] at hprims
   constructor
   · intro h
-    let ⟨h1, h2⟩ := H.bool (oldContains _ primBool h)
-    exact ⟨newContains _ h1, newContains _ h2⟩
-  · intro ci h; apply H.boolFalse; rwa [← same _ primBoolFalse]
-  · intro ci h; apply H.boolTrue; rwa [← same _ primBoolTrue]
+    let ⟨h1, h2⟩ := H.bool (oldContains (hprims (by simp)) h)
+    exact ⟨newContains h1, newContains h2⟩
+  · intro ci h; apply H.boolFalse; rwa [← same (hprims (by simp))]
+  · intro ci h; apply H.boolTrue; rwa [← same (hprims (by simp))]
   · intro h
-    let ⟨h1, h2⟩ := H.nat (oldContains _ primNat h)
-    exact ⟨newContains _ h1, newContains _ h2⟩
-  · intro ci h; apply H.natZero; rwa [← same _ primNatZero]
-  · intro ci h; apply H.natSucc; rwa [← same _ primNatSucc]
-  · intro h a b; exact (H.natAdd (oldContains _ (prim _ (by simp)) h) a b).mono le
-  · intro h a b; exact (H.natSub (oldContains _ (prim _ (by simp)) h) a b).mono le
-  · intro h a b; exact (H.natMul (oldContains _ (prim _ (by simp)) h) a b).mono le
-  · intro h a b; exact (H.natPow (oldContains _ (prim _ (by simp)) h) a b).mono le
-  · intro h a b; exact (H.natGcd (oldContains _ (prim _ (by simp)) h) a b).mono le
-  · intro h a b; exact (H.natMod (oldContains _ (prim _ (by simp)) h) a b).mono le
-  · intro h a b; exact (H.natDiv (oldContains _ (prim _ (by simp)) h) a b).mono le
-  · intro h a b; exact (H.natBEq (oldContains _ (prim _ (by simp)) h) a b).mono le
-  · intro h a b; exact (H.natBLE (oldContains _ (prim _ (by simp)) h) a b).mono le
-  · intro h a b; exact (H.natLAnd (oldContains _ (prim _ (by simp)) h) a b).mono le
-  · intro h a b; exact (H.natLOr (oldContains _ (prim _ (by simp)) h) a b).mono le
-  · intro h a b; exact (H.natXor (oldContains _ (prim _ (by simp)) h) a b).mono le
-  · intro h a b; exact (H.natShiftLeft (oldContains _ (prim _ (by simp)) h) a b).mono le
-  · intro h a b; exact (H.natShiftRight (oldContains _ (prim _ (by simp)) h) a b).mono le
-  · intro ci h; apply H.charOfNat; rwa [← same _ (prim _ (by simp))]
+    let ⟨h1, h2⟩ := H.nat (oldContains (hprims (by simp)) h)
+    exact ⟨newContains h1, newContains h2⟩
+  · intro ci h; apply H.natZero; rwa [← same (hprims (by simp))]
+  · intro ci h; apply H.natSucc; rwa [← same (hprims (by simp))]
+  · intro h a b; exact (H.natAdd (oldContains (hprims (by simp)) h) a b).mono le
+  · intro h a b; exact (H.natSub (oldContains (hprims (by simp)) h) a b).mono le
+  · intro h a b; exact (H.natMul (oldContains (hprims (by simp)) h) a b).mono le
+  · intro h a b; exact (H.natPow (oldContains (hprims (by simp)) h) a b).mono le
+  · intro h a b; exact (H.natGcd (oldContains (hprims (by simp)) h) a b).mono le
+  · intro h a b; exact (H.natMod (oldContains (hprims (by simp)) h) a b).mono le
+  · intro h a b; exact (H.natDiv (oldContains (hprims (by simp)) h) a b).mono le
+  · intro h a b; exact (H.natBEq (oldContains (hprims (by simp)) h) a b).mono le
+  · intro h a b; exact (H.natBLE (oldContains (hprims (by simp)) h) a b).mono le
+  · intro h a b; exact (H.natLAnd (oldContains (hprims (by simp)) h) a b).mono le
+  · intro h a b; exact (H.natLOr (oldContains (hprims (by simp)) h) a b).mono le
+  · intro h a b; exact (H.natXor (oldContains (hprims (by simp)) h) a b).mono le
+  · intro h a b; exact (H.natShiftLeft (oldContains (hprims (by simp)) h) a b).mono le
+  · intro h a b; exact (H.natShiftRight (oldContains (hprims (by simp)) h) a b).mono le
+  · intro ci h; apply H.charOfNat; rwa [← same (hprims (by simp))]
   · intro ci h
-    obtain ⟨rfl, h2, h3⟩ := H.stringOfList (by rwa [← same _ (prim _ (by simp))])
+    obtain ⟨rfl, h2, h3⟩ := H.stringOfList (by rwa [← same (hprims (by simp))])
     exact ⟨rfl, h2.mono le, h3.mono le⟩
 
 theorem VEnv.HasPrimitives.addDefEq {env : VEnv} (H : env.HasPrimitives) :
     (env.addDefEq df).HasPrimitives :=
   { H with
-    natAdd := fun h a b => (H.natAdd h a b).mono VEnv.addDefEq_le
-    natSub := fun h a b => (H.natSub h a b).mono VEnv.addDefEq_le
-    natMul := fun h a b => (H.natMul h a b).mono VEnv.addDefEq_le
-    natPow := fun h a b => (H.natPow h a b).mono VEnv.addDefEq_le
-    natGcd := fun h a b => (H.natGcd h a b).mono VEnv.addDefEq_le
-    natMod := fun h a b => (H.natMod h a b).mono VEnv.addDefEq_le
-    natDiv := fun h a b => (H.natDiv h a b).mono VEnv.addDefEq_le
-    natBEq := fun h a b => (H.natBEq h a b).mono VEnv.addDefEq_le
-    natBLE := fun h a b => (H.natBLE h a b).mono VEnv.addDefEq_le
-    natLAnd := fun h a b => (H.natLAnd h a b).mono VEnv.addDefEq_le
-    natLOr := fun h a b => (H.natLOr h a b).mono VEnv.addDefEq_le
-    natXor := fun h a b => (H.natXor h a b).mono VEnv.addDefEq_le
-    natShiftLeft := fun h a b => (H.natShiftLeft h a b).mono VEnv.addDefEq_le
-    natShiftRight := fun h a b => (H.natShiftRight h a b).mono VEnv.addDefEq_le
-    stringOfList := fun h =>
+    natAdd h a b := (H.natAdd h a b).mono VEnv.addDefEq_le
+    natSub h a b := (H.natSub h a b).mono VEnv.addDefEq_le
+    natMul h a b := (H.natMul h a b).mono VEnv.addDefEq_le
+    natPow h a b := (H.natPow h a b).mono VEnv.addDefEq_le
+    natGcd h a b := (H.natGcd h a b).mono VEnv.addDefEq_le
+    natMod h a b := (H.natMod h a b).mono VEnv.addDefEq_le
+    natDiv h a b := (H.natDiv h a b).mono VEnv.addDefEq_le
+    natBEq h a b := (H.natBEq h a b).mono VEnv.addDefEq_le
+    natBLE h a b := (H.natBLE h a b).mono VEnv.addDefEq_le
+    natLAnd h a b := (H.natLAnd h a b).mono VEnv.addDefEq_le
+    natLOr h a b := (H.natLOr h a b).mono VEnv.addDefEq_le
+    natXor h a b := (H.natXor h a b).mono VEnv.addDefEq_le
+    natShiftLeft h a b := (H.natShiftLeft h a b).mono VEnv.addDefEq_le
+    natShiftRight h a b := (H.natShiftRight h a b).mono VEnv.addDefEq_le
+    stringOfList h :=
       let ⟨h1, h2, h3⟩ := H.stringOfList h
       ⟨h1, h2.mono VEnv.addDefEq_le, h3.mono VEnv.addDefEq_le⟩ }
 
@@ -199,10 +134,9 @@ theorem VEnvs.WF.safePrimitives_add {ves : VEnvs} {env : Environment}
     (wf : ves.WF env) (ci : ConstantInfo)
     (hfresh : env.find? ci.name = none)
     (hok : Environment.primitives.contains ci.name →
-      ci.safety = .safe ∧ ci.levelParams = []) :
-    (env.add ci).find? (n : Name) = some (ci' : ConstantInfo) → Environment.primitives.contains n →
-      ci'.safety = .safe ∧ ci'.levelParams = [] := by
-  intro hfind hp
+      ci.safety = .safe ∧ ci.levelParams = [])
+    (hfind : (env.add ci).find? (n : Name) = some ci')
+    (hp : Environment.primitives.contains n) : ci'.safety = .safe ∧ ci'.levelParams = [] := by
   have mapWF := (wf.tr (safety := .safe)).map_wf
   have hnone : env.constants.find? ci.name = none := by
     rw [← mapWF.find?'_eq_find?]
@@ -211,14 +145,9 @@ theorem VEnvs.WF.safePrimitives_add {ves : VEnvs} {env : Environment}
   change SMap.find?' (env.constants.insert ci.name ci) n = some ci' at hfind
   rw [mapWF'.find?'_eq_find?, mapWF.find?_insert] at hfind
   split at hfind
-  · cases hfind
-    rename_i heq
-    have heq' := LawfulBEq.eq_of_beq heq
-    cases heq'
-    exact hok hp
-  · apply wf.safePrimitives ?_ hp
-    rw [Kernel.Environment.find?, mapWF.find?'_eq_find?]
-    exact hfind
+  · cases hfind; cases LawfulBEq.eq_of_beq ‹_›; exact hok hp
+  · refine wf.safePrimitives ?_ hp
+    rwa [Kernel.Environment.find?, mapWF.find?'_eq_find?]
 
 theorem addConstCore.WF {env : Environment} {ves : VEnvs} (wf : ves.WF env)
     (ci : ConstantInfo) (ci' : VConstVal) (checkSafety : DefinitionSafety)
@@ -237,8 +166,8 @@ theorem addConstCore.WF {env : Environment} {ves : VEnvs} (wf : ves.WF env)
       (ves.venv safety).addConst ci.name ci'.toVConstant = some venv' →
       TrEnv' safety env.constants env.quotInit (ves.venv safety) →
       TrEnv' safety (env.constants.insert ci.name ci) env.quotInit venv') :
-    ∃ ves' : VEnvs, ves'.WF (env.add ci) ∧ ∀ safety, ves.venv safety ≤ ves'.venv safety := by
-  classical
+    ∃ ves' : VEnvs, ves'.WF (env.add ci) ∧
+      ∀ safety, (ves.venv safety).AddConst safety ci ci'.toVConstant (ves'.venv safety) := by
   have hnMap : env.constants.find? ci.name = none := by
     rw [← (wf.tr (safety := .safe)).map_wf.find?'_eq_find?]
     exact hn
@@ -248,53 +177,37 @@ theorem addConstCore.WF {env : Environment} {ves : VEnvs} (wf : ves.WF env)
   have visible_wf (safety) (hvisible : safety ≤ ci.safety) :
       ci'.toVConstant.WF (ves.venv safety) :=
     hci.mono (wf.mono (visible_le safety hvisible))
-  have hex (safety) (hvisible : safety ≤ ci.safety) :=
-    (wf.tr (safety := safety)).exists_addConst hn ci'.toVConstant
-  let next (safety : DefinitionSafety) : VEnv :=
-    if hvisible : safety ≤ ci.safety then Classical.choose (hex safety hvisible)
-    else ves.venv safety
+  have hves' safety : ∃ venv', (ves.venv safety).AddConst safety ci ci'.toVConstant venv' := by
+    unfold VEnv.AddConst; split <;> [rename_i hvisible; exact ⟨ves.venv safety, rfl⟩]
+    have ⟨venv', hadd⟩ := (wf.tr (safety := safety)).exists_addConst hn ci'.toVConstant
+    exact ⟨venv', visible_tr safety hvisible, visible_wf safety hvisible, hadd⟩
+  obtain ⟨ves', hves'⟩ := VEnvs.axiom_of_choice hves'
   have hadd (safety) (hvisible : safety ≤ ci.safety) :
-      (ves.venv safety).addConst ci.name ci'.toVConstant = some (next safety) := by
-    simpa [next, hvisible] using Classical.choose_spec (hex safety hvisible)
-  let ves' : VEnvs := ⟨next⟩
-  refine ⟨ves', ?_, ?_⟩
-  · refine {
-      tr := ?_
-      hasPrimitives := ?_
-      safePrimitives := wf.safePrimitives_add ci hn hprim
-      mono := ?_ }
-    · intro safety
-      change TrEnv' safety (env.constants.insert ci.name ci) env.quotInit (next safety)
+      (ves.venv safety).addConst ci.name ci'.toVConstant = some (ves'.venv safety) := by
+    have h := hves' safety; unfold VEnv.AddConst at h; rw [if_pos hvisible] at h; exact h.2.2
+  have hsame (safety) (hvisible : ¬ safety ≤ ci.safety) : ves'.venv safety = ves.venv safety := by
+    have h := hves' safety; unfold VEnv.AddConst at h; rwa [if_neg hvisible] at h
+  refine ⟨ves', ?_, hves'⟩
+  exact {
+    tr {safety} := by
       by_cases hvisible : safety ≤ ci.safety
       · exact step safety _ (visible_tr safety hvisible) (visible_wf safety hvisible)
           (hadd safety hvisible) (wf.tr (safety := safety))
-      · simpa [next, hvisible] using
-          TrEnv'.ignore (ci := ci) hnMap hvisible (wf.tr (safety := safety))
-    · intro safety
+      · rw [hsame safety hvisible]
+        exact TrEnv'.ignore (ci := ci) hnMap hvisible (wf.tr (safety := safety))
+    hasPrimitives {safety} := by
       by_cases hvisible : safety ≤ ci.safety
-      · exact preserves safety _ hvisible (hadd safety hvisible) wf.hasPrimitives
-      · simpa [ves', next, hvisible] using wf.hasPrimitives (safety := safety)
-    · intro safety safety' hle
-      change next safety' ≤ next safety
+      · exact preserves safety _ hvisible (hadd safety hvisible) (wf.hasPrimitives (safety := safety))
+      · rw [hsame safety hvisible]; exact wf.hasPrimitives (safety := safety)
+    safePrimitives := wf.safePrimitives_add ci hn hprim
+    mono {safety safety'} hle := by
       by_cases hvisible' : safety' ≤ ci.safety
       · have hvisible := DefinitionSafety.le_trans hle hvisible'
-        rw [show next safety' = Classical.choose (hex safety' hvisible') by simp [next, hvisible'],
-          show next safety = Classical.choose (hex safety hvisible) by simp [next, hvisible]]
-        exact VEnv.addConst_mono (wf.mono hle)
-          (Classical.choose_spec (hex safety' hvisible'))
-          (Classical.choose_spec (hex safety hvisible))
-      · rw [show next safety' = ves.venv safety' by simp [next, hvisible']]
-        by_cases hvisible : safety ≤ ci.safety
-        · rw [show next safety = Classical.choose (hex safety hvisible) by simp [next, hvisible]]
-          exact (wf.mono hle).trans
-            (VEnv.addConst_le (Classical.choose_spec (hex safety hvisible)))
-        · rw [show next safety = ves.venv safety by simp [next, hvisible]]
-          exact wf.mono hle
-  · intro safety
-    change ves.venv safety ≤ next safety
-    by_cases hvisible : safety ≤ ci.safety
-    · simpa [next, hvisible] using VEnv.addConst_le (hadd safety hvisible)
-    · simp [next, hvisible, VEnv.LE.rfl]
+        exact VEnv.addConst_mono (wf.mono hle) (hadd safety' hvisible') (hadd safety hvisible)
+      rw [hsame safety' hvisible']
+      by_cases hvisible : safety ≤ ci.safety
+      · exact (wf.mono hle).trans (VEnv.addConst_le (hadd safety hvisible))
+      · rw [hsame safety hvisible]; exact wf.mono hle }
 
 theorem addConst.WF {env : Environment} {ves : VEnvs} (wf : ves.WF env)
     (ci : ConstantInfo) (ci' : VConstVal) (checkSafety : DefinitionSafety)
@@ -309,9 +222,9 @@ theorem addConst.WF {env : Environment} {ves : VEnvs} (wf : ves.WF env)
       (ves.venv safety).addConst ci.name ci'.toVConstant = some venv' →
       TrEnv' safety env.constants env.quotInit (ves.venv safety) →
       TrEnv' safety (env.constants.insert ci.name ci) env.quotInit venv') :
-    ∃ ves' : VEnvs, ves'.WF (env.add ci) ∧ ∀ safety, ves.venv safety ≤ ves'.venv safety := by
-  exact addConstCore.WF wf ci ci' checkSafety visible_le htr hci hn
-    (fun hp => by simp_all)
+    ∃ ves' : VEnvs, ves'.WF (env.add ci) ∧
+      ∀ safety, (ves.venv safety).AddConst safety ci ci'.toVConstant (ves'.venv safety) :=
+  addConstCore.WF wf ci ci' checkSafety visible_le htr hci hn (by simp_all)
     (fun _ _ _ hadd hp => hp.addConst hnonprim hadd) step
 
 theorem addDef.WF {env : Environment} {ves : VEnvs} (wf : ves.WF env)
@@ -327,71 +240,56 @@ theorem addDef.WF {env : Environment} {ves : VEnvs} (wf : ves.WF env)
       (ves.venv safety).addConst v.name ci'.toVConstant = some base →
       (base.addDefEq ci'.toDefEq).HasPrimitives) :
     ∃ ves' : VEnvs, ves'.WF (env.add (.defnInfo v)) ∧
-      ∀ safety, ves.venv safety ≤ ves'.venv safety := by
-  classical
+      ∀ safety, (ves.venv safety).AddDef safety (.defnInfo v) ci' (ves'.venv safety) := by
   have hnMap : env.constants.find? v.name = none := by
-    rw [← (wf.tr (safety := .safe)).map_wf.find?'_eq_find?]
-    exact hn
+    rwa [← (wf.tr (safety := .safe)).map_wf.find?'_eq_find?]
   have visible_tr (safety) (hvisible : safety ≤ (ConstantInfo.defnInfo v).safety) :
-      TrDefVal safety (ves.venv safety) (.defnInfo v) ci' := by
-    have htr' : TrDefVal safety (ves.venv checkSafety) (.defnInfo v) ci' :=
+      TrDefVal safety (ves.venv safety) (.defnInfo v) ci' :=
+    .mono (wf.mono (visible_le safety hvisible)) <|
       ⟨⟨htr.1.1.sf_mono (visible_le safety hvisible), htr.1.2⟩, htr.2⟩
-    exact htr'.mono (wf.mono (visible_le safety hvisible))
-  have visible_wf (safety) (hvisible : safety ≤ (ConstantInfo.defnInfo v).safety) :
-      ci'.WF (ves.venv safety) := hci.mono (wf.mono (visible_le safety hvisible))
-  have hex (safety) (hvisible : safety ≤ (ConstantInfo.defnInfo v).safety) :=
-    (wf.tr (safety := safety)).exists_addConst hn ci'.toVConstant
-  let base (safety : DefinitionSafety) (hvisible : safety ≤ (ConstantInfo.defnInfo v).safety) :=
-    Classical.choose (hex safety hvisible)
-  let next (safety : DefinitionSafety) : VEnv :=
-    if hvisible : safety ≤ (ConstantInfo.defnInfo v).safety then
-      (base safety hvisible).addDefEq ci'.toDefEq
-    else ves.venv safety
-  have hadd (safety) (hvisible : safety ≤ (ConstantInfo.defnInfo v).safety) :
-      (ves.venv safety).addConst v.name ci'.toVConstant = some (base safety hvisible) :=
-    Classical.choose_spec (hex safety hvisible)
-  let ves' : VEnvs := ⟨next⟩
-  refine ⟨ves', ?_, ?_⟩
-  · refine {
-      tr := ?_
-      hasPrimitives := ?_
-      safePrimitives := wf.safePrimitives_add (.defnInfo v) hn hprim
-      mono := ?_ }
-    · intro safety
-      change TrEnv' safety (env.constants.insert v.name (.defnInfo v)) env.quotInit (next safety)
+  have visible_wf safety hvisible := hci.mono (wf.mono (visible_le safety hvisible))
+  have hves' safety : ∃ venv', (ves.venv safety).AddDef safety (.defnInfo v) ci' venv' := by
+    unfold VEnv.AddDef; split <;> [rename_i hvisible; exact ⟨ves.venv safety, rfl⟩]
+    have ⟨base, hadd⟩ := (wf.tr (safety := safety)).exists_addConst hn ci'.toVConstant
+    exact ⟨base.addDefEq ci'.toDefEq,
+      base, visible_tr safety hvisible, visible_wf safety hvisible, hadd, rfl⟩
+  obtain ⟨ves', hves'⟩ := VEnvs.axiom_of_choice hves'
+  have hbase (safety) (hvisible : safety ≤ (ConstantInfo.defnInfo v).safety) :
+      ∃ base, (ves.venv safety).addConst v.name ci'.toVConstant = some base ∧
+        ves'.venv safety = base.addDefEq ci'.toDefEq := by
+    have h := hves' safety; unfold VEnv.AddDef at h; rw [if_pos hvisible] at h
+    obtain ⟨base, _, _, hadd, heq⟩ := h; exact ⟨base, hadd, heq⟩
+  have hsame (safety) (hvisible : ¬ safety ≤ (ConstantInfo.defnInfo v).safety) :
+      ves'.venv safety = ves.venv safety := by
+    have h := hves' safety; unfold VEnv.AddDef at h; rwa [if_neg hvisible] at h
+  refine ⟨ves', ?_, hves'⟩
+  refine {
+    tr {safety} := by
+      change TrEnv' safety (env.constants.insert v.name (.defnInfo v)) env.quotInit _
       by_cases hvisible : safety ≤ (ConstantInfo.defnInfo v).safety
-      · simpa [next, hvisible] using TrEnv'.defn (visible_tr safety hvisible)
+      · obtain ⟨base, hadd, heq⟩ := hbase safety hvisible
+        exact heq ▸ TrEnv'.defn (visible_tr safety hvisible)
           (by rwa [← (wf.tr (safety := safety)).map_wf.find?'_eq_find?])
-          (visible_wf safety hvisible) (hadd safety hvisible) (wf.tr (safety := safety))
-      · simpa [next, hvisible, ConstantInfo.name, ConstantInfo.toConstantVal] using
+          (visible_wf safety hvisible) hadd (wf.tr (safety := safety))
+      · rw [hsame safety hvisible]
+        simpa [ConstantInfo.name, ConstantInfo.toConstantVal] using
           TrEnv'.ignore (ci := .defnInfo v) hnMap hvisible (wf.tr (safety := safety))
-    · intro safety
+    hasPrimitives {safety} := by
       by_cases hvisible : safety ≤ (ConstantInfo.defnInfo v).safety
-      · simpa [ves', next, hvisible] using preserves safety (base safety hvisible)
-          hvisible (hadd safety hvisible)
-      · simpa [ves', next, hvisible] using wf.hasPrimitives (safety := safety)
-    · intro safety safety' hle
-      change next safety' ≤ next safety
+      · obtain ⟨base, hadd, heq⟩ := hbase safety hvisible
+        rw [heq]; exact preserves safety base hvisible hadd
+      · rw [hsame safety hvisible]; exact wf.hasPrimitives (safety := safety)
+    safePrimitives := wf.safePrimitives_add (.defnInfo v) hn hprim
+    mono {safety safety'} hle := by
       by_cases hvisible' : safety' ≤ (ConstantInfo.defnInfo v).safety
       · have hvisible := DefinitionSafety.le_trans hle hvisible'
-        rw [show next safety' = (base safety' hvisible').addDefEq ci'.toDefEq by
-              simp [next, hvisible'],
-          show next safety = (base safety hvisible).addDefEq ci'.toDefEq by
-              simp [next, hvisible]]
-        exact VEnv.addDefEq_mono <| VEnv.addConst_mono (wf.mono hle)
-          (hadd safety' hvisible') (hadd safety hvisible)
-      · rw [show next safety' = ves.venv safety' by simp [next, hvisible']]
-        by_cases hvisible : safety ≤ (ConstantInfo.defnInfo v).safety
-        · rw [show next safety = (base safety hvisible).addDefEq ci'.toDefEq by
-              simp [next, hvisible]]
-          exact (wf.mono hle).trans <| (VEnv.addConst_le (hadd safety hvisible)).trans
-            VEnv.addDefEq_le
-        · rw [show next safety = ves.venv safety by simp [next, hvisible]]
-          exact wf.mono hle
-  · intro safety
-    change ves.venv safety ≤ next safety
-    by_cases hvisible : safety ≤ (ConstantInfo.defnInfo v).safety
-    · rw [show next safety = (base safety hvisible).addDefEq ci'.toDefEq by
-          simp [next, hvisible]]
-      exact (VEnv.addConst_le (hadd safety hvisible)).trans VEnv.addDefEq_le
-    · simp [next, hvisible, VEnv.LE.rfl]
+        obtain ⟨base', hadd', heq'⟩ := hbase safety' hvisible'
+        obtain ⟨base, hadd, heq⟩ := hbase safety hvisible
+        rw [heq', heq]
+        exact VEnv.addDefEq_mono <| VEnv.addConst_mono (wf.mono hle) hadd' hadd
+      rw [hsame safety' hvisible']
+      by_cases hvisible : safety ≤ (ConstantInfo.defnInfo v).safety
+      · obtain ⟨base, hadd, heq⟩ := hbase safety hvisible
+        rw [heq]
+        exact (wf.mono hle).trans <| (VEnv.addConst_le hadd).trans VEnv.addDefEq_le
+      · rw [hsame safety hvisible]; exact wf.mono hle }
